Add new approach

ShadowInterpMatchCoind.v
@@ -1,4 +1,5 @@
-From Coq Require Import PArith Arith Lia String List.
+From Coq Require Import Utf8 Arith Lia String List.
+From Paco Require Import paco.
 Import ListNotations.
 
 Local Open Scope string_scope.
@@ -6,905 +7,742 @@ Local Unset Elimination Schemes.
 Local Set Primitive Projections.
 
 Definition var := string.
-Definition loc := positive.
 
-Inductive tm :=
-  | Var (x : var)
-  | Fn (x : var) (e : tm) (* λ x . e *)
-  | App (f a : tm)
-  | Link (m e : tm) (* m ⋊ e *)
-  | Mt (* ε *)
-  | Bind (x : var) (v m : tm) (* let rec x = v ; m *)
-  | Zero (* O *)
-  | Succ (n : tm) (* S n *)
-  | Case (e : tm) (z : tm) (n : var) (s : tm)
-    (* match e with 0 => z | S n => s end *)
-.
+Module simple.
 
-Inductive shdw {wvl} :=
-  | Init
-  | Read (s : shdw) (x : var)
-  | Call (s : shdw) (w : wvl)
-  | SuccS (s : shdw)
-  | PredS (s : shdw)
+Inductive shdw {vl} :=
+  | Rd (x : var)
+  | Ap (s : shdw) (v : vl)
 .
 
 Arguments shdw : clear implicits.
 
-Definition predS {wvl} (s : shdw wvl) :=
-  match s with
-  | Init | Read _ _ | Call _ _ | PredS _ => PredS s
-  | SuccS s => s
-  end.
-
-Inductive nv {wvl} :=
-  | nv_mt (* • *)
-  | nv_sh (s : shdw wvl) (* [s] *)
-  | nv_bd (x : var) (w : wvl) (σ : nv) (* bound value *)
+Inductive nv {vl} :=
+  | Init
+  | nv_mt
+  | nv_bd (x : var) (v : vl) (σ : nv)
 .
 
 Arguments nv : clear implicits.
 
-Inductive vl {wvl K} :=
-  | vl_exp (σ : nv wvl)
-  | vl_sh (s : shdw wvl) (* s *)
-  | vl_clos (x : var) (k : K) (σ : nv wvl)
-  | vl_nat (n : nat)
+Inductive vl {tr} :=
+  | vl_sh (s : shdw vl) (* s *)
+  | vl_clos (x : var) (t : tr) (σ : nv vl) (* ⟨ λx.t, σ ⟩ *)
 .
 
 Arguments vl : clear implicits.
 
-Inductive wvl {K} :=
-  | wvl_v (v : vl wvl K) (* v *)
-  | wvl_recv (v : vl wvl K) (* μ.v *)
-  | wvl_bloc (n : nat) (* bound location *)
-  | wvl_floc (ℓ : loc) (* free location *)
-.
+Section link.
+  Context {trace : Type}.
+  Let value := vl trace.
+  Let shadow := shdw value.
+  Let env := nv value.
 
-Arguments wvl : clear implicits.
+  Definition rd x :=
+    fix rd (σ : env) :=
+      match σ with
+      | Init => Some (vl_sh (Rd x))
+      | nv_mt => None
+      | nv_bd x' v σ' =>
+        if x =? x' then Some v else rd σ'
+      end.
+
+  Definition link_shdw stuck link_value link_trace (σ0 : env) :=
+    fix link (s : shadow) k : trace :=
+      match s with
+      | Rd x =>
+        match rd x σ0 with
+        | None => stuck
+        | Some v => k v
+        end
+      | Ap s' v =>
+        let k_s f :=
+          let k_v a :=
+            match f with
+            | vl_sh f' => k (vl_sh (Ap f' a))
+            | vl_clos x k' σ => link_trace (nv_bd x a σ) k' k
+            end
+          in link_value v k_v
+        in link s' k_s
+      end.
+
+  Definition link_nv link_value (σ0 : env) :=
+    fix link (σ : env) k : trace :=
+      match σ with
+      | Init => k σ0
+      | nv_mt => k nv_mt
+      | nv_bd x v σ' =>
+        let k_v v' :=
+          let k_σ σ'' := k (nv_bd x v' σ'')
+          in link σ' k_σ
+        in link_value v k_v
+      end.
+
+  Definition link_vl stuck link_trace (σ0 : env) :=
+    fix link (v : value) k : trace :=
+      match v with
+      | vl_sh s => link_shdw stuck link link_trace σ0 s k
+      | vl_clos x t σ =>
+        let k_σ σ' := k (vl_clos x t σ')
+        in link_nv link σ0 σ k_σ
+      end.
+End link.
 
 Variant traceF {trace} :=
-  | Error
-  | Wal (w : wvl trace)
-  | Match (s : shdw (wvl trace)) (zt : trace) (st : trace)
-  | Guard (σ : nv (wvl trace)) (t : trace)
+  | Stuck
+  | Ret (v : vl trace)
+  | Step (s : nv (vl trace)) (k : trace)
 .
 
 Arguments traceF : clear implicits.
 
-CoInductive trace := mkTrace { _obs_tr : traceF trace }.
+(* Finite approximation *)
+Inductive trace' := mkTrace' (k : traceF trace').
+Definition obs_tr' (t : trace') :=
+  match t with
+  | mkTrace' k => k
+  end.
 
-Definition walue := wvl trace.
-Definition value := vl walue trace.
-Definition shadow := shdw walue.
-Definition env := nv walue.
+(* Infinite tree *)
+CoInductive trace := mkTrace { obs_tr : traceF trace }.
 
-Notation obs_tr t := (_obs_tr t) (only parsing).
-Notation error := (mkTrace Error) (only parsing).
-Notation wal w := (mkTrace (Wal w)) (only parsing).
-Notation case s zt st := (mkTrace (Match s zt st)) (only parsing).
-Notation guard σ t := (mkTrace (Guard σ t)) (only parsing).
+Definition value' := vl trace'.
+Definition value := vl trace.
+Definition shadow' := shdw value'.
+Definition shadow := shdw value.
+Definition env' := nv value'.
+Definition env := nv value.
 
-Section PRE_VAL_IND.
-  Context {K : Type}.
-  Context (Pwvl : wvl K -> Prop) (Pnv : nv (wvl K) -> Prop) (Pvl : vl (wvl K) K -> Prop) (Pshdw : shdw (wvl K) -> Prop).
-  Context (Pwvl_v : forall v, Pvl v -> Pwvl (wvl_v v))
-          (Pwvl_recv : forall v, Pvl v -> Pwvl (wvl_recv v))
-          (Pwvl_bloc : forall n, Pwvl (wvl_bloc n))
-          (Pwvl_floc : forall ℓ, Pwvl (wvl_floc ℓ)).
-  Context (Pnv_mt : Pnv nv_mt)
-          (Pnv_sh : forall s, Pshdw s -> Pnv (nv_sh s))
-          (Pnv_bd : forall x w σ, Pwvl w -> Pnv σ -> Pnv (nv_bd x w σ)).
-  Context (Pvl_exp : forall σ, Pnv σ -> Pvl (vl_exp σ))
-          (Pvl_sh : forall s, Pshdw s -> Pvl (vl_sh s))
-          (Pvl_clos : forall x k σ, Pnv σ -> Pvl (vl_clos x k σ))
-          (Pvl_nat : forall n, Pvl (vl_nat n)).
+Notation stuck' := (mkTrace' Stuck) (only parsing).
+Notation stuck := (mkTrace Stuck) (only parsing).
+Notation ret' v := (mkTrace' (Ret v)) (only parsing).
+Notation ret v := (mkTrace (Ret v)) (only parsing).
+Notation step' σ k := (mkTrace' (Step σ k)) (only parsing).
+Notation step σ k := (mkTrace (Step σ k)) (only parsing).
+
+Fixpoint link_trace n σ0 (t : trace) k :=
+  match n with
+  | 0 => stuck
+  | S n' =>
+    match obs_tr t with
+    | Stuck => stuck
+    | Ret v => link_vl stuck (link_trace n') σ0 v k
+    | Step σ t' =>
+      let k_σ σ' := step σ' (link_trace n' σ0 t' k)
+      in link_nv (link_vl stuck (link_trace n') σ0) σ0 σ k_σ
+    end
+  end.
+
+Fixpoint link_trace' n σ0 (t : trace') k :=
+  match n with
+  | 0 => stuck'
+  | S n' =>
+    match obs_tr' t with
+    | Stuck => stuck'
+    | Ret v => link_vl stuck' (link_trace' n') σ0 v k
+    | Step σ t' =>
+      let k_σ σ' := step' σ' (link_trace' n' σ0 t' k)
+      in link_nv (link_vl stuck' (link_trace' n') σ0) σ0 σ k_σ
+    end
+  end.
+
+Definition link_value n := link_vl stuck (link_trace n).
+Definition link_value' n := link_vl stuck' (link_trace' n).
+Definition link_env n σ0 := link_nv (link_value n σ0) σ0.
+Definition link_env' n σ0 := link_nv (link_value' n σ0) σ0.
+Definition link_shadow n σ0 := link_shdw stuck (link_value n σ0) (link_trace n) σ0.
+Definition link_shadow' n σ0 := link_shdw stuck' (link_value' n σ0) (link_trace' n) σ0.
+
+Inductive term :=
+  | Var (x : var)
+  | Lam (x : var) (t : term)
+  | App (fn arg : term)
+.
+
+Definition sem :=
+  fix sem (t : term) k : nat → trace :=
+  match t with
+  | Var x => fun _ =>
+    let r := vl_sh (Rd x)
+    in step Init (k r)
+  | Lam x e => fun n =>
+    let r := vl_clos x (sem e (fun r => ret r) n) Init
+    in step Init (k r)
+  | App fn arg => fun n =>
+    let k_fn f :=
+      let k_arg a :=
+        match f with
+        | vl_sh f' => k (vl_sh (Ap f' a))
+        | vl_clos x k' σ => link_trace n (nv_bd x a σ) k' k
+        end
+      in sem arg k_arg n
+    in step Init (sem fn k_fn n)
+  end.
+
+Definition sem' :=
+  fix sem (t : term) k : nat → trace' :=
+  match t with
+  | Var x => fun _ =>
+    let r := vl_sh (Rd x)
+    in step' Init (k r)
+  | Lam x e => fun n =>
+    let r := vl_clos x (sem e (fun r => ret' r) n) Init
+    in step' Init (k r)
+  | App fn arg => fun n =>
+    let k_fn f :=
+      let k_arg a :=
+        match f with
+        | vl_sh f' => k (vl_sh (Ap f' a))
+        | vl_clos x k' σ => link_trace' n (nv_bd x a σ) k' k
+        end
+      in sem arg k_arg n
+    in step' Init (sem fn k_fn n)
+  end.
+
+Definition ω := Lam "x" (App (Var "x") (Var "x")).
+Compute sem' (App ω ω) (fun r => ret' r) 10.
+End simple.
+
+Inductive shdw {nv wvl} :=
+  | Init
+  | Rd (s : shdw) (σ : nv) (x : var)
+  | Ap (s : shdw) (w : wvl)
+.
+
+Arguments shdw : clear implicits.
+
+Inductive nv {wvl} :=
+  | nv_sh (s : shdw nv wvl) (* [s] *)
+  | nv_one (x : var) (w : wvl) (* x ↦ w *)
+  | nv_mrg (σ σ' : nv) (* σ ;; σ' *)
+.
+
+Arguments nv : clear implicits.
+
+Variant vl {P wvl tr} :=
+  | vl_prim (p : P) (* primitive value *)
+  | vl_nv (σ : nv wvl)
+  | vl_sh (s : shdw (nv wvl) wvl) (* s *)
+  | vl_clos (x : var) (t : tr) (σ : nv wvl) (* ⟨ λx.t, σ ⟩ *)
+.
+
+Arguments vl : clear implicits.
+
+Inductive wvl {P L tr} :=
+  | wvl_v (v : vl P wvl tr) (* v *)
+  | wvl_recv (v : L → vl P wvl tr) (* μℓ.v *)
+  | wvl_loc (ℓ : L) (* free location *)
+.
+
+Arguments wvl : clear implicits.
+
+Variant traceF {P L trace} :=
+  | Stuck
+  | Ret (w : wvl P L trace)
+  | Step (σ : nv (wvl P L trace)) (t : trace)
+.
+
+Arguments traceF : clear implicits.
+
+(* Finite approximation *)
+Inductive trace' {P L} := mkTrace' (k : traceF P L trace').
+Definition obs_tr' {P L} (t : @trace' P L) :=
+  match t with
+  | mkTrace' k => k
+  end.
+
+(* Infinite tree *)
+CoInductive trace {P L} := mkTrace { obs_tr : traceF P L trace }.
+
+Arguments trace' : clear implicits.
+Arguments trace : clear implicits.
+Arguments mkTrace {_ _} _.
+
+Definition walue' P L := wvl P L (trace' P L).
+Definition walue P L := wvl P L (trace P L).
+Definition env' P L := nv (walue' P L).
+Definition env P L := nv (walue P L).
+Definition shadow' P L := shdw (env' P L) (walue' P L).
+Definition shadow P L := shdw (env' P L) (walue P L).
+Definition value' P L := vl P (walue' P L) (trace' P L).
+Definition value P L := vl P (walue P L) (trace P L).
+
+Notation stuck' := (mkTrace' Stuck) (only parsing).
+Notation stuck := (mkTrace Stuck) (only parsing).
+Notation ret' w := (mkTrace' (Ret w)) (only parsing).
+Notation ret w := (mkTrace (Ret w)) (only parsing).
+Notation step' σ t := (mkTrace' (Step σ t)) (only parsing).
+Notation step σ t := (mkTrace (Step σ t)) (only parsing).
+
+Section ind.
+  Context {P L tr : Type}.
+  Let Walue := wvl P L tr.
+  Let Value := vl P Walue tr.
+  Let Env := nv Walue.
+  Let Shadow := shdw Env Walue.
+  Context (Ptr : tr → Prop) (tr_ind : ∀ k, Ptr k)
+          (Pshdw : Shadow → Prop)
+          (Pnv : Env → Prop)
+          (Pvl : Value → Prop)
+          (Pwvl : Walue → Prop).
   Context (PInit : Pshdw Init)
-          (PRead : forall s x, Pshdw s -> Pshdw (Read s x))
-          (PCall : forall s w, Pshdw s -> Pwvl w -> Pshdw (Call s w))
-          (PSucc : forall s, Pshdw s -> Pshdw (SuccS s))
-          (PPred : forall s, Pshdw s -> Pshdw (PredS s)).
+          (PRd : ∀ s σ x, Pshdw s → Pnv σ → Pshdw (Rd s σ x))
+          (PAp : ∀ s w, Pshdw s → Pwvl w → Pshdw (Ap s w)).
+  Context (Pnv_sh : ∀ s, Pshdw s → Pnv (nv_sh s))
+          (Pnv_one : ∀ x w, Pwvl w → Pnv (nv_one x w))
+          (Pnv_mrg : ∀ σ σ', Pnv σ → Pnv σ' -> Pnv (nv_mrg σ σ')).
+  Context (Pvl_prim : ∀ p, Pvl (vl_prim p))
+          (Pvl_nv : ∀ σ, Pnv σ → Pvl (vl_nv σ))
+          (Pvl_sh : ∀ s, Pshdw s → Pvl (vl_sh s))
+          (Pvl_clos : ∀ x k σ, Ptr k → Pnv σ → Pvl (vl_clos x k σ)).
+  Context (Pwvl_v : ∀ v, Pvl v → Pwvl (wvl_v v))
+          (Pwvl_recv : ∀ v, (∀ ℓ, Pvl (v ℓ)) → Pwvl (wvl_recv v))
+          (Pwvl_loc : ∀ ℓ, Pwvl (wvl_loc ℓ)).
 
-  Definition shdw_ind wvl_ind :=
-    fix shdw_ind s : Pshdw s :=
-    match s with
-    | Init => PInit
-    | Read s x => PRead s x (shdw_ind s)
-    | Call s w => PCall s w (shdw_ind s) (wvl_ind w)
-    | SuccS s => PSucc s (shdw_ind s)
-    | PredS s => PPred s (shdw_ind s)
-    end.
+  Definition shdw_ind nv_ind wvl_ind :=
+    fix go s : Pshdw s :=
+      match s as s' return Pshdw s' with
+      | Init => PInit
+      | Rd s σ x => PRd s σ x (go s) (nv_ind σ)
+      | Ap f w => PAp f w (go f) (wvl_ind w)
+      end.
 
   Definition nv_ind wvl_ind :=
-    fix nv_ind σ : Pnv σ :=
-    match σ with
-    | nv_mt => Pnv_mt
-    | nv_sh s => Pnv_sh s (shdw_ind wvl_ind s)
-    | nv_bd x w σ => Pnv_bd x w σ (wvl_ind w) (nv_ind σ)
-    end.
+    fix go σ : Pnv σ :=
+      match σ as σ' return Pnv σ' with
+      | nv_sh s => Pnv_sh s (shdw_ind go wvl_ind s)
+      | nv_one x w => Pnv_one x w (wvl_ind w)
+      | nv_mrg σ1 σ2 => Pnv_mrg σ1 σ2 (go σ1) (go σ2)
+      end.
 
-  Definition vl_ind (wvl_ind : forall w, Pwvl w) : forall v, Pvl v.
-  Proof.
-    refine (
-    let shdw_ind := shdw_ind wvl_ind in
-    let nv_ind := nv_ind wvl_ind in
-    fix vl_ind v :=
-    match v with
-    | vl_exp σ => Pvl_exp σ (nv_ind σ)
-    | vl_sh s => Pvl_sh s (shdw_ind s)
-    | vl_clos x k σ => Pvl_clos x k σ (nv_ind σ)
-    | vl_nat n => Pvl_nat n
-    end).
-  Defined.
+  Definition vl_ind wvl_ind v : Pvl v :=
+    match v as v' return Pvl v' with
+    | vl_prim p => Pvl_prim p
+    | vl_nv σ => Pvl_nv σ (nv_ind wvl_ind σ)
+    | vl_sh s => Pvl_sh s (shdw_ind (nv_ind wvl_ind) wvl_ind s)
+    | vl_clos x t σ => Pvl_clos x t σ (tr_ind t) (nv_ind wvl_ind σ)
+    end.
 
   Fixpoint wvl_ind w : Pwvl w :=
     match w with
     | wvl_v v => Pwvl_v v (vl_ind wvl_ind v)
-    | wvl_recv v => Pwvl_recv v (vl_ind wvl_ind v)
-    | wvl_bloc n => Pwvl_bloc n
-    | wvl_floc ℓ => Pwvl_floc ℓ
+    | wvl_recv v => Pwvl_recv v (fun ℓ => vl_ind wvl_ind (v ℓ))
+    | wvl_loc ℓ => Pwvl_loc ℓ
     end.
 
   Lemma pre_val_ind :
-    (forall w, Pwvl w) /\
-    (forall σ, Pnv σ) /\
-    (forall v, Pvl v) /\
-    (forall s, Pshdw s).
+    (∀ s, Pshdw s) ∧ (∀ σ, Pnv σ) ∧ (∀ v, Pvl v) ∧ (∀ w, Pwvl w).
   Proof.
-    eauto using wvl_ind, (nv_ind wvl_ind), (vl_ind wvl_ind), (shdw_ind wvl_ind).
+    pose proof (nv_ind wvl_ind).
+    pose proof (vl_ind wvl_ind).
+    pose proof (shdw_ind (nv_ind wvl_ind) wvl_ind).
+    eauto using wvl_ind.
   Qed.
-End PRE_VAL_IND.
+End ind.
 
-Module ValNotations.
-(* Printing *)
-  Notation " 'μ' v " := (wvl_recv v) (at level 60, right associativity, only printing).
-  Notation " v " := (wvl_v v) (at level 60, right associativity, only printing).
-  Notation " n " := (wvl_bloc n) (at level 60, right associativity, only printing).
-  Notation " ℓ " := (wvl_floc ℓ) (at level 60, right associativity, only printing).
+Section trace'_ind.
+  Context {P L : Type}.
+  Let tr := trace' P L.
+  Let Walue := wvl P L tr.
+  Let Value := vl P Walue tr.
+  Let Env := nv Walue.
+  Let Shadow := shdw Env Walue.
+  Context (Ptr : tr → Prop)
+          (Pshdw : Shadow → Prop)
+          (Pnv : Env → Prop)
+          (Pvl : Value → Prop)
+          (Pwvl : Walue → Prop).
+  Context (PInit : Pshdw Init)
+          (PRd : ∀ s σ x, Pshdw s → Pnv σ → Pshdw (Rd s σ x))
+          (PAp : ∀ s w, Pshdw s → Pwvl w → Pshdw (Ap s w)).
+  Context (Pnv_sh : ∀ s, Pshdw s → Pnv (nv_sh s))
+          (Pnv_one : ∀ x w, Pwvl w → Pnv (nv_one x w))
+          (Pnv_mrg : ∀ σ σ', Pnv σ → Pnv σ' -> Pnv (nv_mrg σ σ')).
+  Context (Pvl_prim : ∀ p, Pvl (vl_prim p))
+          (Pvl_nv : ∀ σ, Pnv σ → Pvl (vl_nv σ))
+          (Pvl_sh : ∀ s, Pshdw s → Pvl (vl_sh s))
+          (Pvl_clos : ∀ x k σ, Ptr k → Pnv σ → Pvl (vl_clos x k σ)).
+  Context (Pwvl_v : ∀ v, Pvl v → Pwvl (wvl_v v))
+          (Pwvl_recv : ∀ v, (∀ ℓ, Pvl (v ℓ)) → Pwvl (wvl_recv v))
+          (Pwvl_loc : ∀ ℓ, Pwvl (wvl_loc ℓ)).
+  Context (Pstuck : Ptr stuck')
+          (Pret : ∀ w, Pwvl w → Ptr (ret' w))
+          (Pstep : ∀ σ t, Pnv σ → Ptr t → Ptr (step' σ t)).
 
-  Notation " s " := (vl_sh s) (at level 60, right associativity, only printing).
-  Notation " σ " := (vl_exp σ) (at level 60, right associativity, only printing).
-  Notation " n " := (vl_nat n) (at level 60, right associativity, only printing).
-  Notation "'⟨' 'λ' x k σ '⟩'" := (vl_clos x k σ) (at level 60, right associativity, only printing).
+  Check shdw_ind.
+  Fixpoint trace'_ind (t : tr) : Ptr t :=
+    let wvl_ind' := wvl_ind _ trace'_ind _ _ _ _
+      PInit PRd PAp
+      Pnv_sh Pnv_one Pnv_mrg
+      Pvl_prim Pvl_nv Pvl_sh Pvl_clos
+      Pwvl_v Pwvl_recv Pwvl_loc in
+    let nv_ind' := nv_ind _ _ _
+      PInit PRd PAp
+      Pnv_sh Pnv_one Pnv_mrg wvl_ind' in
+    match t with
+    | mkTrace' k =>
+      match k as k' return Ptr (mkTrace' k') with
+      | Stuck => Pstuck
+      | Ret w => Pret w (wvl_ind' w)
+      | Step σ t => Pstep σ t (nv_ind' σ) (trace'_ind t)
+      end
+    end.
 
-  Notation "•" := (nv_mt) (at level 60, right associativity, only printing).
-  Notation "'⟪' s '⟫'" := (nv_sh s) (at level 60, right associativity, only printing).
-  Notation "'⟪' x ',' w '⟫' ';;' σ " := (nv_bd x w σ) (at level 60, right associativity, only printing).
+  Lemma val'_ind :
+    (∀ s, Pshdw s) ∧ (∀ σ, Pnv σ) ∧ (∀ v, Pvl v) ∧ (∀ w, Pwvl w) ∧ (∀ t, Ptr t).
+  Proof.
+    pose proof
+      (pre_val_ind (tr := tr) (L := L) Ptr trace'_ind Pshdw Pnv Pvl Pwvl
+        PInit PRd PAp
+        Pnv_sh Pnv_one Pnv_mrg
+        Pvl_prim Pvl_nv Pvl_sh Pvl_clos
+        Pwvl_v Pwvl_recv Pwvl_loc).
+    intuition auto.
+    apply trace'_ind.
+  Qed.
+End trace'_ind.
 
-  Notation "⊥" := (Error) (at level 60, right associativity, only printing).
-  Notation "w" := (Wal w) (at level 60, right associativity, only printing).
-  Notation "s '→' b" := (Match s b) (at level 60, right associativity, only printing).
-  Notation "σ '→' t" := (Guard σ t) (at level 60, right associativity, only printing).
-End ValNotations.
+Section map.
+  Definition map_shdw {wvl wvl'}
+    (map_wvl : wvl → wvl')
+    (map_nv : nv wvl → nv wvl') :=
+    fix map_s (s : shdw (nv wvl) wvl) : shdw (nv wvl') wvl' :=
+      match s with
+      | Init => Init
+      | Rd s' σ x => Rd (map_s s') (map_nv σ) x
+      | Ap f w => Ap (map_s f) (map_wvl w)
+      end.
 
-(** Operations for substitution *)
-(* open the bound location i with ℓ *)
-Definition open_loc_shdw f (i : nat) (ℓ : loc) :=
-  fix open (s : shadow) : shadow :=
-  match s with
-  | Init => Init
-  | Read s x => Read (open s) x
-  | Call s w => Call (open s) (f i ℓ w)
-  | SuccS s => SuccS (open s)
-  | PredS s => PredS (open s)
-  end.
+  Definition map_nv {wvl wvl'}
+    (map_wvl : wvl → wvl') :=
+    fix map_nv (σ : nv wvl) : nv wvl' :=
+      match σ with
+      | nv_sh s => nv_sh (map_shdw map_wvl map_nv s)
+      | nv_one x w => nv_one x (map_wvl w)
+      | nv_mrg σ1 σ2 => nv_mrg (map_nv σ1) (map_nv σ2)
+      end.
 
-Definition open_loc_nv f (i : nat) (ℓ : loc) :=
-  fix open (σ : env) :=
-  match σ with
-  | nv_mt => nv_mt
-  | nv_sh s => nv_sh (open_loc_shdw f i ℓ s)
-  | nv_bd x w σ' =>
-    nv_bd x (f i ℓ w) (open σ')
-  end.
+  Definition map_vl {P wvl wvl' tr tr'}
+    (map_wvl : wvl → wvl')
+    (map_tr : tr → tr')
+    (v : vl P wvl tr) : vl P wvl' tr' :=
+    match v with
+    | vl_prim p => vl_prim p
+    | vl_nv σ => vl_nv (map_nv map_wvl σ)
+    | vl_sh s => vl_sh (map_shdw map_wvl (map_nv map_wvl) s)
+    | vl_clos x t σ => vl_clos x (map_tr t) (map_nv map_wvl σ)
+    end.
 
-Definition open_loc_vl f (i : nat) (ℓ : loc) :=
-  fix open (v : value) :=
-  match v with
-  | vl_exp σ => vl_exp (open_loc_nv f i ℓ σ)
-  | vl_sh s => vl_sh (open_loc_shdw f i ℓ s)
-  | vl_clos x k σ => vl_clos x k (open_loc_nv f i ℓ σ)
-  | vl_nat n => vl_nat n
-  end.
+  Definition map_wvl {P L tr tr'}
+    (map_tr : tr → tr') :=
+    fix map_w (w : wvl P L tr) : wvl P L tr' :=
+      match w with
+      | wvl_v v => wvl_v (map_vl map_w map_tr v)
+      | wvl_recv v => wvl_recv (fun ℓ => map_vl map_w map_tr (v ℓ))
+      | wvl_loc ℓ => wvl_loc ℓ
+      end.
+End map.
 
-Fixpoint open_loc_walue (i : nat) (ℓ : loc) (w : walue) : walue :=
-  let open_loc_vl := open_loc_vl open_loc_walue in
-  let open_loc_shdw := open_loc_shdw open_loc_walue in
-  match w with
-  | wvl_v v => wvl_v (open_loc_vl i ℓ v)
-  | wvl_recv v => wvl_recv (open_loc_vl (S i) ℓ v)
-  | wvl_bloc n => if Nat.eqb i n then wvl_floc ℓ else wvl_bloc n
-  | wvl_floc ℓ => wvl_floc ℓ
-  end.
+Section rel.
+  Definition rel_shdw {wvl wvl'}
+    (rel_wvl : wvl → wvl' → Prop)
+    (rel_nv : nv wvl → nv wvl' → Prop) :=
+    fix rel_s (s : shdw (nv wvl) wvl) (s' : shdw (nv wvl') wvl') : Prop :=
+      match s with
+      | Init => match s' with Init => True | _ => False end
+      | Rd s σ x =>
+        match s' with
+        | Rd s' σ' x' => rel_s s s' ∧ rel_nv σ σ' ∧ x = x'
+        | _ => False
+        end
+      | Ap f w =>
+        match s' with
+        | Ap f' w' => rel_s f f' ∧ rel_wvl w w'
+        | _ => False
+        end
+      end.
 
-Definition open_loc_value := open_loc_vl open_loc_walue.
-Definition open_loc_env := open_loc_nv open_loc_walue.
-Definition open_loc_shadow := open_loc_shdw open_loc_walue.
+  Definition rel_nv {wvl wvl'}
+    (rel_wvl : wvl → wvl' → Prop) :=
+    fix rel_nv (σ : nv wvl) (σ' : nv wvl') : Prop :=
+      match σ with
+      | nv_sh s =>
+        match σ' with
+        | nv_sh s' => rel_shdw rel_wvl rel_nv s s'
+        | _ => False
+        end
+      | nv_one x w =>
+        match σ' with
+        | nv_one x' w' => x = x' ∧ rel_wvl w w'
+        | _ => False
+        end
+      | nv_mrg σ1 σ2 =>
+        match σ' with
+        | nv_mrg σ1' σ2' => rel_nv σ1 σ1' ∧ rel_nv σ2 σ2'
+        | _ => False
+        end
+      end.
 
-(* close the free location ℓ with the binding depth i *)
-Definition close_shdw f (i : nat) (ℓ : loc) :=
-  fix close (s : shadow) : shadow :=
-  match s with
-  | Init => Init
-  | Read s x => Read (close s) x
-  | Call s w => Call (close s) (f i ℓ w)
-  | SuccS s => SuccS (close s)
-  | PredS s => PredS (close s)
-  end.
+  Definition rel_vl {P wvl wvl' tr tr'}
+    (rel_wvl : wvl → wvl' → Prop)
+    (rel_tr : tr → tr' → Prop)
+    (v : vl P wvl tr) (v' : vl P wvl' tr') :=
+    match v with
+    | vl_prim p =>
+      match v' with
+      | vl_prim p' => p = p'
+      | _ => False
+      end
+    | vl_nv σ =>
+      match v' with
+      | vl_nv σ' => rel_nv rel_wvl σ σ'
+      | _ => False
+      end
+    | vl_sh s =>
+      match v' with
+      | vl_sh s' => rel_shdw rel_wvl (rel_nv rel_wvl) s s'
+      | _ => False
+      end
+    | vl_clos x t σ =>
+      match v' with
+      | vl_clos x' t' σ' =>
+        x = x' ∧ rel_tr t t' ∧ rel_nv rel_wvl σ σ'
+      | _ => False
+      end
+    end.
 
-Definition close_nv f (i : nat) (ℓ : loc) :=
-  fix close (σ : env) : env :=
-  match σ with
-  | nv_mt => nv_mt
-  | nv_sh s => nv_sh (close_shdw f i ℓ s)
-  | nv_bd x w σ' =>
-    nv_bd x (f i ℓ w) (close σ')
-  end.
+  Definition rel_wvl {P L tr tr'}
+    (rel_tr : tr → tr' → Prop) :=
+    fix rel_w (w : wvl P L tr) (w' : wvl P L tr') :=
+      match w with
+      | wvl_v v =>
+        match w' with
+        | wvl_v v' => rel_vl rel_w rel_tr v v'
+        | _ => False
+        end
+      | wvl_recv v =>
+        match w' with
+        | wvl_recv v' => ∀ ℓ, rel_vl rel_w rel_tr (v ℓ) (v' ℓ)
+        | _ => False
+        end
+      | wvl_loc ℓ => match w' with wvl_loc ℓ' => ℓ = ℓ' | _ => False end
+      end.
 
-Definition close_vl f (i : nat) (ℓ : loc) :=
-  fix close (v : value) : value :=
-  match v with
-  | vl_exp σ => vl_exp (close_nv f i ℓ σ)
-  | vl_sh s => vl_sh (close_shdw f i ℓ s)
-  | vl_clos x k σ => vl_clos x k (close_nv f i ℓ σ)
-  | vl_nat n => vl_nat n
-  end.
+  Context {P L tr tr' : Type}
+    (r r' : tr → tr' → Prop)
+    (LEt : ∀ t t', r t t' → r' t t').
 
-Fixpoint close_walue (i : nat) (ℓ : loc) (w : walue) : walue :=
-  let close_vl := close_vl close_walue in
-  let close_shdw := close_shdw close_walue in
-  match w with
-  | wvl_v v => wvl_v (close_vl i ℓ v)
-  | wvl_recv v => wvl_recv (close_vl (S i) ℓ v)
-  | wvl_bloc n => wvl_bloc n
-  | wvl_floc ℓ' => if Pos.eqb ℓ ℓ' then wvl_bloc i else wvl_floc ℓ'
-  end.
+  Definition rel_shdw_monotone (s : shdw (nv (wvl P L tr)) (wvl P L tr)) :=
+    ∀ s', rel_shdw (rel_wvl r) (rel_nv (rel_wvl r)) s s' →
+          rel_shdw (rel_wvl r') (rel_nv (rel_wvl r')) s s'
+  .
+  Definition rel_nv_monotone (σ : nv (wvl P L tr)) :=
+    ∀ σ', rel_nv (rel_wvl r) σ σ' → rel_nv (rel_wvl r') σ σ'
+  .
+  Definition rel_vl_monotone (v : vl P (wvl P L tr) tr) :=
+    ∀ v', rel_vl (rel_wvl r) r v v' → rel_vl (rel_wvl r') r' v v'
+  .
+  Definition rel_wvl_monotone (w : wvl P L tr) :=
+    ∀ w', rel_wvl r w w' → rel_wvl r' w w'
+  .
 
-Definition close_value := close_vl close_walue.
-Definition close_env := close_nv close_walue.
-Definition close_shadow := close_shdw close_walue.
+  Lemma rel_monotone :
+    (∀ s, rel_shdw_monotone s) ∧
+    (∀ σ, rel_nv_monotone σ) ∧
+    (∀ v, rel_vl_monotone v) ∧
+    (∀ w, rel_wvl_monotone w).
+  Proof.
+    apply (pre_val_ind _ (fun _ => I));
+    cbv [rel_shdw_monotone rel_nv_monotone rel_vl_monotone rel_wvl_monotone];
+    simpl; intros;
+    match goal with
+    | _ : match ?x with _ => _ end |- _ =>
+      destruct x; intuition auto
+    end.
+  Qed.
+End rel.
 
-(* open the bound location i with u *)
-Definition open_wvl_shdw f (i : nat) (u : walue) :=
-  fix open (s : shadow) : shadow :=
-  match s with
-  | Init => Init
-  | Read s x => Read (open s) x
-  | Call s w => Call (open s) (f i u w)
-  | SuccS s => SuccS (open s)
-  | PredS s => PredS (open s)
-  end.
+(* partial order between finite approximations *)
+Definition le_trace' {P L} :=
+  fix le_t (t t' : trace' P L) :=
+    let le_wvl := rel_wvl le_t in
+    match obs_tr' t with
+    | Stuck => True
+    | Ret w =>
+      match obs_tr' t' with
+      | Ret w' => le_wvl w w'
+      | _ => False
+      end
+    | Step σ k =>
+      match obs_tr' t' with
+      | Step σ' k' => rel_nv le_wvl σ σ' ∧ le_t k k'
+      | _ => False
+      end
+    end.
 
-Definition open_wvl_nv f (i : nat) (u : walue) :=
-  fix open (σ : env) :=
-  match σ with
-  | nv_mt => nv_mt
-  | nv_sh s => nv_sh (open_wvl_shdw f i u s)
-  | nv_bd x w σ' =>
-    nv_bd x (f i u w) (open σ')
-  end.
+Lemma le_trace'_refl {P L} :
+  let le_wvl (w : walue' P L) := rel_wvl le_trace' w in
+  let le_vl (v : value' P L) := rel_vl le_wvl le_trace' v in
+  let le_nv (σ : env' P L) := rel_nv le_wvl σ in
+  let le_shdw (s : shadow' P L) := rel_shdw le_wvl le_nv s in
+  (∀ s, le_shdw s s) ∧
+  (∀ σ, le_nv σ σ) ∧
+  (∀ v, le_vl v v) ∧
+  (∀ w, le_wvl w w) ∧
+  (∀ t : trace' P L, le_trace' t t).
+Proof. cbn zeta. apply val'_ind; simpl; auto. Qed.
 
-Definition open_wvl_vl f (i : nat) (u : walue) :=
-  fix open (v : value) :=
-  match v with
-  | vl_exp σ => vl_exp (open_wvl_nv f i u σ)
-  | vl_sh s => vl_sh (open_wvl_shdw f i u s)
-  | vl_clos x k σ => vl_clos x k (open_wvl_nv f i u σ)
-  | vl_nat n => vl_nat n
-  end.
-
-Fixpoint open_wvl_walue (i : nat) (u : walue) (w : walue) : walue :=
-  let open_wvl_vl := open_wvl_vl open_wvl_walue in
-  let open_wvl_shdw := open_wvl_shdw open_wvl_walue in
-  match w with
-  | wvl_v v => wvl_v (open_wvl_vl i u v)
-  | wvl_recv v => wvl_recv (open_wvl_vl (S i) u v)
-  | wvl_bloc n => if Nat.eqb i n then u else wvl_bloc n
-  | wvl_floc ℓ => wvl_floc ℓ
-  end.
-
-Definition open_wvl_value := open_wvl_vl open_wvl_walue.
-Definition open_wvl_env := open_wvl_nv open_wvl_walue.
-Definition open_wvl_shadow := open_wvl_shdw open_wvl_walue.
-
-(* allocate fresh locations *)
-Definition alloc_shdw f :=
-  fix alloc (s : shadow) : positive :=
-  match s with
-  | Init => xH
-  | Read s x => alloc s
-  | Call s w => Pos.max (alloc s) (f w)
-  | SuccS s => alloc s
-  | PredS s => alloc s
-  end.
-
-Definition alloc_nv f :=
-  fix alloc (σ : env) : positive :=
-  match σ with
-  | nv_mt => xH
-  | nv_sh s => alloc_shdw f s
-  | nv_bd _ w σ' => Pos.max (f w) (alloc σ')
-  end.
-
-Definition alloc_vl f :=
-  fix alloc (v : value) : positive :=
-  match v with
-  | vl_exp σ | vl_clos _ _ σ => alloc_nv f σ
-  | vl_sh s => alloc_shdw f s
-  | vl_nat n => xH
-  end.
-
-Fixpoint alloc_walue (w : walue) : positive :=
-  let alloc_vl := alloc_vl alloc_walue in
-  let alloc_shdw := alloc_shdw alloc_walue in
-  match w with
-  | wvl_v v | wvl_recv v => alloc_vl v
-  | wvl_bloc _ => 1
-  | wvl_floc ℓ => Pos.succ ℓ
-  end%positive.
-
-Definition alloc_value := alloc_vl alloc_walue.
-Definition alloc_env := alloc_nv alloc_walue.
-Definition alloc_shadow := alloc_shdw alloc_walue.
-
-(* term size *)
-Definition size_shdw f :=
-  fix size (s : shadow) :=
-  match s with
-  | Init => O
-  | Read s x => S (size s)
-  | Call s w => S (Nat.max (size s) (f w))
-  | SuccS s => S (size s)
-  | PredS s => S (size s)
-  end.
-
-Definition size_nv f :=
-  fix size (σ : env) :=
-  match σ with
-  | nv_mt => O
-  | nv_sh s => S (size_shdw f s)
-  | nv_bd _ w σ' => S (Nat.max (f w) (size σ'))
-  end.
-
-Definition size_vl f :=
-  fix size (v : value) :=
-  match v with
-  | vl_exp σ | vl_clos _ _ σ => S (size_nv f σ)
-  | vl_sh s => S (size_shdw f s)
-  | vl_nat _ => O
-  end.
-
-Fixpoint size_walue (w : walue) :=
-  let size_vl := size_vl size_walue in
-  let size_shdw := size_shdw size_walue in
-  match w with
-  | wvl_v v | wvl_recv v => S (size_vl v)
-  | wvl_bloc _ | wvl_floc _ => O
-  end.
-
-Definition size_value := size_vl size_walue.
-Definition size_env := size_nv size_walue.
-Definition size_shadow := size_shdw size_walue.
-
-Definition open_loc_size_eq_wvl w :=
-  forall n ℓ, size_walue w = size_walue (open_loc_walue n ℓ w).
-Definition open_loc_size_eq_nv σ :=
-  forall n ℓ, size_env σ = size_env (open_loc_env n ℓ σ).
-Definition open_loc_size_eq_vl v :=
-  forall n ℓ, size_value v = size_value (open_loc_value n ℓ v).
-Definition open_loc_size_eq_shdw s :=
-  forall n ℓ, size_shadow s = size_shadow (open_loc_shadow n ℓ s).
-
-Lemma open_loc_size_eq :
-  (forall w, open_loc_size_eq_wvl w) /\
-  (forall σ, open_loc_size_eq_nv σ) /\
-  (forall v, open_loc_size_eq_vl v) /\
-  (forall s, open_loc_size_eq_shdw s).
+Lemma le_trace'_trans {P L} :
+  let le_wvl (w : walue' P L) := rel_wvl le_trace' w in
+  let le_vl (v : value' P L) := rel_vl le_wvl le_trace' v in
+  let le_nv (σ : env' P L) := rel_nv le_wvl σ in
+  let le_shdw (s : shadow' P L) := rel_shdw le_wvl le_nv s in
+  (∀ s' : shadow' P L,
+    ∀ s s'', le_shdw s s' → le_shdw s' s'' → le_shdw s s'') ∧
+  (∀ σ' : env' P L,
+    ∀ σ σ'', le_nv σ σ' → le_nv σ' σ'' → le_nv σ σ'') ∧
+  (∀ v' : value' P L,
+    ∀ v v'', le_vl v v' → le_vl v' v'' → le_vl v v'') ∧
+  (∀ w' : walue' P L,
+    ∀ w w'', le_wvl w w' → le_wvl w' w'' → le_wvl w w'') ∧
+  (∀ t' : trace' P L,
+    ∀ t t'', le_trace' t t' → le_trace' t' t'' → le_trace' t t'').
 Proof.
-  apply pre_val_ind; repeat intro; simpl; auto.
+  cbn zeta. apply val'_ind; simpl; intros;
   match goal with
-  | |- context [Nat.eqb ?x ?y] => destruct (Nat.eqb x y)
-  end; simpl; auto.
+  | |- rel_shdw _ _ ?s ?s'' =>
+    destruct s; simpl in *; intuition eauto;
+    subst; destruct s''; intuition eauto
+  | |- rel_nv _ ?σ ?σ'' =>
+    destruct σ; simpl in *; intuition eauto;
+    subst; destruct σ''; intuition eauto
+  | |- rel_vl _ _ ?v ?v'' =>
+    destruct v; simpl in *; intuition eauto;
+    subst; destruct v''; intuition eauto
+  | |- rel_wvl _ ?w ?w'' =>
+    destruct w; simpl in *; intuition eauto;
+    subst; destruct w''; intuition eauto
+  | |- le_trace' ?t ?t'' =>
+    destruct t; simpl in *; intuition eauto;
+    subst; destruct t''; intuition eauto
+  end.
+  - destruct k; simpl in *; intuition eauto.
+  - destruct k; simpl in *; intuition eauto.
+    destruct k0; simpl in *; intuition eauto.
+  - destruct k; simpl in *; intuition eauto.
+    destruct k0; simpl in *; intuition eauto.
 Qed.
 
-Definition read_env (σ : env) (x : var) :=
-  let fix read σ (acc : env -> env) :=
-    match σ with
-    | nv_mt => None
-    | nv_sh s => Some (wvl_v (vl_sh (Read s x)), acc nv_mt)
-    | nv_bd x' w' σ' =>
-      if x =? x' then Some (w', acc σ') else
-      let acc' σ' := acc (nv_bd x' w' σ')
-      in read σ' acc'
-    end
-  in read σ id.
-
-Definition unroll (w : walue) : option value :=
-  match w with
-  | wvl_v v => Some v
-  | wvl_recv v => Some (open_wvl_value 0 w v)
-  | wvl_bloc _ | wvl_floc _ => None
-  end.
-
-Definition bind (k : walue -> trace) : trace -> trace :=
-  cofix bind_ t :=
-    match obs_tr t with
-    | Error => error
-    | Wal w => k w
-    | Match s zt st => case s (bind_ zt) (bind_ st)
-    | Guard σ t => guard σ (bind_ t)
+(* approx t' t : t' is a finite approximation of t *)
+Definition approx {P L} :=
+  fix approx (t' : trace' P L) (t : trace P L) :=
+    let approx_w := rel_wvl approx in
+    match obs_tr' t' with
+    | Stuck => True
+    | Ret w' =>
+      match obs_tr t with
+      | Ret w => approx_w w' w
+      | _ => False
+      end
+    | Step σ' k' =>
+      match obs_tr t with
+      | Step σ k => rel_nv approx_w σ' σ ∧ approx k' k
+      | _ => False
+      end
     end.
 
-CoFixpoint link (σ0 : env) (t : trace) : trace.
+Variant eq_traceF {P L} eq : trace P L → trace P L → Prop :=
+  | eq_stuck : eq_traceF eq stuck stuck
+  | eq_ret w w'
+    (EQw : rel_wvl eq w w')
+  : eq_traceF eq (ret w) (ret w')
+  | eq_step σ σ' k k'
+    (EQσ : rel_nv (rel_wvl eq) σ σ')
+    (EQk : eq k k')
+  : eq_traceF eq (step σ k) (step σ' k')
+.
+
+Arguments eq_traceF : clear implicits.
+
+Lemma eq_traceF_monotone {P L} : monotone2 (eq_traceF P L).
 Proof.
-  destruct (obs_tr t); cycle 3.
-  - pose (check_guard w :=
-      match unroll w with
-      | Some (vl_sh s) => guard (nv_sh s) (link σ0 t)
-      | Some (vl_exp σ) => guard σ (link σ0 t)
-      | _ => error
-      end).
-    refine (guard nv_mt (bind check_guard _)).
-    refine (link σ0 _).
-    Guarded.
-:=
-  match obs_tr t with
-  | Error => error
-  | Wal (wvl_v v) => wal (wvl_v v)
-  | Wal (wvl_recv v) => wal (wvl_recv v)
-  | Wal (wvl_bloc n) => error
-  | Wal (wvl_floc ℓ) => wal (wvl_floc ℓ)
-  | Match s zt st =>
-    let check_match w :=
-      match unroll w with
-      | Some (vl_sh (SuccS s)) => guard nv_mt (link k σ0 st)
-      | Some (vl_sh s) => case s (link k σ0 zt) (link k σ0 st)
-      | Some (vl_nat O) => guard nv_mt (link k σ0 zt)
-      | Some (vl_nat (S _)) => guard nv_mt (link k σ0 st)
-      | _ => error
-      end
-    in link check_match σ0 (wal (wvl_v (vl_sh s)))
-  | Guard σ t =>
-    let check_guard w :=
-      match unroll w with
-      | Some (vl_sh s) => guard (nv_sh s) (link k σ0 t)
-      | Some (vl_exp σ) => guard σ (link k σ0 t)
-      | _ => error
-      end
-    in link check_guard σ0 (wal (wvl_v (vl_exp σ)))
+  repeat intro. inversion IN; try constructor; subst; auto.
+  all: eapply rel_monotone; eauto.
+Qed.
+
+Hint Resolve eq_traceF_monotone : paco.
+Definition eq_trace P L := paco2 (eq_traceF P L) bot2.
+
+Fixpoint nth_trace {P L} (n : nat) (t : trace P L) : trace' P L :=
+  match n with
+  | 0 => stuck'
+  | S n' =>
+    match obs_tr t with
+    | Stuck => stuck'
+    | Ret w =>
+      let w' := map_wvl (nth_trace n') w in
+      ret' w'
+    | Step σ k =>
+      let σ' := map_nv (map_wvl (nth_trace n')) σ in
+      step' σ' (nth_trace n' k)
+    end
   end.
 
-Definition link_trace (link : walue -> trace) (k : walue -> trace) : trace -> trace :=
-  cofix link_trace_ t :=
-    match obs_tr t with
-    | Error => error
-    | Wal w => bind k (link w)
-    | Match s zt st =>
-      let check_match w :=
-        match unroll w with
-        | Some (vl_sh (SuccS s)) => guard nv_mt (link_trace_ st)
-        | Some (vl_sh s) => case s (link_trace_ zt) (link_trace_ st)
-        | Some (vl_nat O) => guard nv_mt (link_trace_ zt)
-        | Some (vl_nat (S _)) => guard nv_mt (link_trace_ st)
-        | _ => error
-        end
-      in bind check_match (link (wvl_v (vl_sh s)))
-    | Guard σ t =>
-      let check_guard w :=
-        match unroll w with
-        | Some (vl_sh s) => guard (nv_sh s) (link_trace_ t)
-        | Some (vl_exp σ) => guard σ (link_trace_ t)
-        | _ => error
-        end
-      in bind check_guard (link (wvl_v (vl_exp σ)))
+Section flatten.
+  Context {P L : Type} (flatten_walue' : walue' P (walue' P L) → walue' P L).
+ 
+  Definition flatten_shadow' flatten_env' :=
+    fix flatten (s : shadow' P (walue' P L)) : shadow' P L :=
+    match s with
+    | Init => Init
+    | Rd s σ x => Rd (flatten s) (flatten_env' σ) x
+    | Ap s w => Ap (flatten s) (flatten_walue' w)
     end.
 
-Definition read_trace x :=
-  let read w :=
-    match unroll w with
-    | Some (vl_sh s) => wal (wvl_v (vl_sh (Read s x)))
-    | Some (vl_exp σ) =>
-      match read_env σ x with
-      | Some (w, σ) => guard σ (wal w)
-      | None => error
-      end
-    | _ => error
-    end
-  in bind read.
+  Fixpoint flatten_env' (σ : env' P (walue' P L)) : env' P L :=
+    match σ with
+    | nv_sh s => nv_sh (flatten_shadow' flatten_env' s)
+    | nv_one x w => nv_one x (flatten_walue' w)
+    | nv_mrg σ σ' => nv_mrg (flatten_env' σ) (flatten_env' σ')
+    end.
 
-Definition call_trace (link : env -> walue -> trace) (fn arg : trace) : trace :=
-  let check_fn fn :=
-    match unroll fn with
-    | Some (vl_sh s) =>
-      let check_arg arg := wal (wvl_v (vl_sh (Call s arg)))
-      in bind check_arg arg
-    | Some (vl_clos x t σ) =>
-      let check_arg arg := link_trace (link (nv_bd x arg σ)) wal t
-      in bind check_arg arg
-    | _ => error
-    end
-  in bind check_fn fn.
+  Context (flatten_trace' : trace' P (walue' P L) → trace' P L).
 
-Definition close_rec ℓ :=
-  let close w :=
-    match unroll w with
-    | Some v => wal (wvl_recv (close_value 0 ℓ v))
-    | None => error
-    end
-  in bind close.
-
-Definition bd_trace x (w : trace) (σ : trace) :=
-  let check_bd w :=
-    let check_mod σ :=
-      match unroll σ with
-      | Some (vl_sh s) => wal (wvl_v (vl_exp (nv_bd x w (nv_sh s))))
-      | Some (vl_exp σ) => wal (wvl_v (vl_exp (nv_bd x w σ)))
-      | _ => error
-      end
-    in bind check_mod σ
-  in bind check_bd w.
-
-Definition clos_trace x t :=
-  let clos w :=
-    match unroll w with
-    | Some (vl_sh s) => wal (wvl_v (vl_clos x t (nv_sh s)))
-    | Some (vl_exp σ) => wal (wvl_v (vl_clos x t σ))
-    | _ => error
-    end
-  in bind clos.
-
-Definition filter_env :=
-  let filter w :=
-    match unroll w with
-    | Some (vl_sh s) => wal (wvl_v (vl_exp (nv_sh s)))
-    | Some (vl_exp σ) => wal (wvl_v (vl_exp σ))
-    | _ => error
-    end
-  in bind filter.
-
-Definition succ_trace :=
-  let succ w :=
-    match unroll w with
-    | Some (vl_sh s) => wal (wvl_v (vl_sh (SuccS s)))
-    | Some (vl_nat n) => wal (wvl_v (vl_nat (S n)))
-    | _ => error
-    end
-  in bind succ.
-
-Definition pred_trace :=
-  let pred w :=
-    match unroll w with
-    | Some (vl_sh s) => wal (wvl_v (vl_sh (predS s)))
-    | Some (vl_nat (S n)) => wal (wvl_v (vl_nat n))
-    | _ => error
-    end
-  in bind pred.
-
-Definition link_shdw (link : env -> walue -> trace) (σ0 : env) (s : shadow) : trace :=
-  let link_shdw s := link σ0 (wvl_v (vl_sh s)) in
-  let link_wvl w := link σ0 w in
-  match s with
-  | Init => wal (wvl_v (vl_exp σ0))
-  | Read s x => read_trace x (link_shdw s)
-  | Call s w => call_trace link (link_shdw s) (link_wvl w)
-  | SuccS s => succ_trace (link_shdw s)
-  | PredS s => pred_trace (link_shdw s)
-  end.
-
-Definition link_nv (link : env -> walue -> trace) (σ0 : env) (σ : env) : trace :=
-  let link_shdw s := link_shdw link σ0 s in
-  let link_nv σ := link σ0 (wvl_v (vl_exp σ)) in
-  let link_wvl w := link σ0 w in
-  match σ with
-  | nv_mt => wal (wvl_v (vl_exp nv_mt))
-  | nv_sh s => filter_env (link_shdw s)
-  | nv_bd x w σ' => bd_trace x (link_wvl w) (link_nv σ')
-  end.
-
-Definition link_vl (link : env -> walue -> trace) (σ0 : env) v : trace :=
-  let link_shdw s := link_shdw link σ0 s in
-  let link_nv σ := link_nv link σ0 σ in
-  match v with
-  | vl_clos x t σ => clos_trace x t (link_nv σ)
-  | vl_exp σ => link_nv σ
-  | vl_sh s => link_shdw s
-  | vl_nat n => wal (wvl_v (vl_nat n))
-  end.
-
-Definition link_wvl (link : env -> walue -> trace) (σ0 : env) w : trace :=
-  let link_shdw s := link_shdw link σ0 s in
-  let link_nv σ := link_nv link σ0 σ in
-  let link_vl v := link_vl link σ0 v in
-  match w with
-  | wvl_v v => link_vl v
-  | wvl_recv v =>
-    let ℓ := Pos.max (alloc_value v) (alloc_env σ0) in
-    close_rec ℓ (link_vl (open_loc_value 0 ℓ v))
-  | wvl_bloc n => error
-  | wvl_floc ℓ => wal (wvl_floc ℓ)
-  end.
-
-Local Unset Guard Checking.
-CoFixpoint link := link_wvl link.
-Local Set Guard Checking.
-
-CoFixpoint link' (σ0 : env) (w : walue) : trace :=
-  match w with
-  | wvl_v v =>
+  Definition flatten_value' (v : value' P (walue' P L)) : value' P L :=
     match v with
+    | vl_prim p => vl_prim p
+    | vl_nv σ => vl_nv (flatten_env' σ)
+    | vl_sh s => vl_sh (flatten_shadow' flatten_env' s)
     | vl_clos x t σ =>
-      match σ with
-      | nv_mt => clos_trace x t (wal (wvl_v (vl_exp nv_mt)))
-      | nv_sh s =>
-        match s with
-        | Init => clos_trace x t (wal (wvl_v (vl_exp σ0)))
-        | Read s x =>
-          read_trace x (guard nv_mt (link' σ0 (wvl_v (vl_sh s))))
-        | Call s w =>
-          call_trace link' (link' σ0 (wvl_v (vl_sh s))) (link' σ0 w)
-        | SuccS s => succ_trace (link' σ0 (wvl_v (vl_sh s)))
-        | PredS s => pred_trace (link' σ0 (wvl_v (vl_sh s)))
-        end
-      | nv_bd x w σ => bd_trace x (link' σ0 w) (link' σ0 (wvl_v (vl_exp σ)))
-      end
-    | vl_exp σ => error
-    | vl_sh s => error
-    | vl_nat n => error
-    end
-  | _ => error
+      vl_clos x
+        (flatten_trace' t)
+        (flatten_env' σ)
+    end.
+End flatten.
+
+Definition flatten_walue' {P L} flatten_trace' :=
+  fix flatten_walue' (w : walue' P (walue' P L)) : walue' P L :=
+  let f := flatten_value' flatten_walue' flatten_trace' in
+  match w with
+  | wvl_v v => wvl_v (f v)
+  | wvl_recv v => wvl_recv (fun ℓ => f (v (wvl_loc ℓ)))
+  | wvl_loc ℓ => ℓ (* flatten *)
   end.
 
-Definition sem_link (link : env -> walue -> trace) (σ w : trace) :=
-  let check_module m :=
-    match unroll m with
-    | Some (vl_sh s) => link_trace (link (nv_sh s)) wal w
-    | Some (vl_exp σ) => link_trace (link σ) wal w
-    | _ => error
-    end
-  in bind check_module σ.
-
-(* precondition : bd, exp has no free locations *)
-Definition sem_bind (link : env -> walue -> trace) x (bd exp : trace) :=
-  let check_bd w :=
-    match unroll w with
-    | Some v =>
-      let w := wvl_recv (close_value 0 xH v) in
-      let check_exp σ :=
-        match unroll σ with
-        | Some (vl_sh s) => wal (wvl_v (vl_exp (nv_bd x w (nv_sh s))))
-        | Some (vl_exp σ) => wal (wvl_v (vl_exp (nv_bd x w σ)))
-        | _ => error
-        end
-      in link_trace (link (nv_bd x w (nv_sh Init))) check_exp exp
-    | None => error
-    end
-  in link_trace (link (nv_bd x (wvl_floc xH) (nv_sh Init))) check_bd bd.
-
-Definition sem_case (link : env -> walue -> trace) (m zt : trace) x (st : trace) :=
-  let check_match m :=
-    match unroll m with
-    | Some (vl_sh (SuccS s)) =>
-      link_trace (link (nv_bd x (wvl_v (vl_sh s)) (nv_sh Init))) wal st
-    | Some (vl_sh s) =>
-      let st := link_trace (link (nv_bd x (wvl_v (vl_sh (PredS s))) (nv_sh Init))) wal st in
-      case s zt st
-    | Some (vl_nat 0) => zt
-    | Some (vl_nat (S n)) =>
-      link_trace (link (nv_bd x (wvl_v (vl_nat n)) (nv_sh Init))) wal st
-    | _ => error
-    end
-  in bind check_match m.
-
-Definition eval (link : env -> walue -> trace) :=
-  fix eval (e : tm) : trace :=
-  match e with
-  | Var x => wal (wvl_v (vl_sh (Read Init x)))
-  | Fn x M => wal (wvl_v (vl_clos x (eval M) (nv_sh Init)))
-  | App M N => call_trace link (eval M) (eval N)
-  | Link M N => sem_link link (eval M) (eval N)
-  | Mt => guard (nv_sh Init) (wal (wvl_v (vl_exp nv_mt)))
-  | Bind x M N => sem_bind link x (eval M) (eval N)
-  | Zero => wal (wvl_v (vl_nat 0))
-  | Succ n => succ_trace (eval n)
-  | Case m z x s => sem_case link (eval m) (eval z) x (eval s)
-  end.
-
-Definition interp := eval link.
-Definition ω := Fn "x" (App (Var "x") (Var "x")).
-Definition test :=
-  Eval cbn in
-    obs_tr (interp (App ω ω)).
-Import ValNotations.
-Print test.
-(* examples *)
-Fixpoint get_wal t :=
+Definition flatten_trace' {P L} :=
+  fix flatten_trace' (t : trace' P (walue' P L)) : trace' P L :=
+  let f := flatten_walue' flatten_trace' in
   match t with
-  | Bot => []
-  | Wal w => [w]
-  | Match _ b =>
-    let fold acc (b : cstr_type * trace) :=
-      let (c, t) := b in get_wal t ++ acc
-    in List.fold_left fold b nil
-  | Guard _ t => get_wal t
-  end%list.
-
-Definition zero_tm c :=
-  Cstr {|
-    cs_type := {| cs_name := c; cs_arity := 0 |};
-    cs_args := []%vec;
-  |}.
-Definition succ_tm t :=
-  Cstr {|
-    cs_type := {| cs_name := Succ; cs_arity := 1 |};
-    cs_args := [t]%vec;
-  |}.
-Definition one_tm := succ_tm (zero_tm Zero).
-Definition two_tm := succ_tm one_tm.
-Definition three_tm := succ_tm two_tm.
-(* Fixpoint add m n := match m with 0 => n | S m => S (add m n) end *)
-Definition zero_branch (t : tm) :=
-  {|
-    br_cstr := {| cs_name := Zero; cs_arity := _ |};
-    br_vars := []%vec;
-    br_body := t
-  |}.
-Definition succ_branch x (t : tm) :=
-  {|
-    br_cstr := {| cs_name := Succ; cs_arity := _ |};
-    br_vars := [x]%vec;
-    br_body := t
-  |}.
-
-Module SimpleExamples.
-Definition pred_tm :=
-  Fn "n" (Case (Var "n") [zero_branch (zero_tm Zero); succ_branch "m" (Var "m")])
-.
-
-Definition add_tm :=
-Link (Bind "+"
-  (Fn "m"
-    (Fn "n"
-      (Case (Var "m")
-        [zero_branch (Var "n");
-        succ_branch "m" (succ_tm (App (App (Var "+") (Var "m")) (Var "n")))]
-      )))
-  Mt) (Var "+")
-.
-
-Definition mult_tm :=
-Link (Bind "×"
-  (Fn "m"
-    (Fn "n"
-      (Case (Var "m")
-        [zero_branch (Var "m");
-        succ_branch "m"
-        (App
-          (App add_tm (Var "n"))
-          (App
-            (App (Var "×") (Var "m"))
-            (Var "n")))])))
-  Mt) (Var "×")
-.
-
-Definition infinity :=
-Link (Bind "n" (succ_tm (Var "n")) Mt)
-  (Var "n").
-
-Definition three_plus_three := App (App add_tm three_tm) three_tm.
-Definition three_times_three := App (App mult_tm three_tm) three_tm.
-
-Definition x_plus_three := App (App add_tm three_tm) (Var "x").
-
-Definition double_x := App (App add_tm (Var "x")) (Var "x").
-
-Compute get_wal (interp 5 three_plus_three).
-Compute get_wal (interp 10 three_times_three).
-Compute get_wal (interp 6 x_plus_three).
-Compute get_wal (interp 6 double_x).
-Compute get_wal (interp 6 (App pred_tm infinity)).
-
-Compute get_wal (interp 100
-  (App
-    (App add_tm
-      (App
-        (App add_tm one_tm)
-        two_tm))
-    (Var "x"))).
-
-Definition sum_tm :=
-Link (Bind "Σ"
-  (Fn "f"
-    (Fn "n"
-      (Case (Var "n")
-        [zero_branch (App (Var "f") (zero_tm Zero));
-        succ_branch "n"
-        (App
-          (App (Var "+") (App (Var "f") (succ_tm (Var "n"))))
-          (App
-            (App (Var "Σ") (Var "f"))
-            (Var "n")))])))
-  Mt) (Var "Σ").
-
-Definition unknown_function :=
-  App (App sum_tm (Var "f")) three_tm.
-
-Compute interp 5 unknown_function.
-
-Definition unknown_function_and_number :=
-  App (App sum_tm (Var "f")) (Var "n").
-
-Definition export_function_number :=
-  Bind "f" (Fn "n" (App (App add_tm (Var "n")) one_tm))
-    (Bind "n" three_tm
-      (Bind "+" add_tm Mt)).
-
-Definition export_function_number_sem :=
-  Eval vm_compute in
-  interp 4 export_function_number.
-
-Definition unknown_function_and_number_sem :=
-  Eval vm_compute in
-  interp 10 unknown_function_and_number.
-
-Compute get_wal (sem_link (link 10)
-  export_function_number_sem
-  unknown_function_and_number_sem).
-
-Compute
-  let l := get_wal (interp 10
-    (Fn "n" (App (App add_tm (Var "n")) one_tm)))
-  in
-  let for_each w :=
-    match w with
-    | wvl_v (vl_clos _ k _) => get_wal k
-    | _ => []
+  | mkTrace' k =>
+    match k with
+    | Stuck => stuck'
+    | Ret w => ret' (f w)
+    | Step σ t => step' (flatten_env' f σ) (flatten_trace' t)
     end
-  in List.map for_each l.
+  end.
 
-Definition ω := Fn "x" (App (Var "x") (Var "x")).
-Definition bomb := Bind "w" ω Mt.
-Definition bomber := Bind "div" (App (Var "w") (Var "w")) Mt.
-Compute interp 10 (Link bomb (Link bomber Mt)).
-Compute interp 10 (Link (Link bomb bomber) Mt).
-End SimpleExamples.
-
-Module MutExample.
-(* even? n = 1 if n is even 0 if n is odd *)
-Definition top_module :=
-Bind "Top"
-  (Bind "Even"
-    (Bind "even?"
-      (Fn "x"
-        (Case (Var "x")
-          [zero_branch one_tm;
-          succ_branch "n" (App (Link (Var "Top") (Link (Var "Odd") (Var "odd?"))) (Var "n"))]
-        ))
-      Mt)
-    (Bind "Odd"
-      (Bind "odd?"
-        (Fn "y"
-          (Case (Var "y")
-            [zero_branch (zero_tm Zero);
-            succ_branch "n" (App (Link (Var "Top") (Link (Var "Even") (Var "even?"))) (Var "n"))]
-          ))
-        Mt)
-      Mt))
-  Mt.
-
-Definition test_even :=
-  Link top_module
-    (Link (Var "Top") (Link (Var "Even") (Var "even?"))).
-Definition test_odd :=
-  Link top_module
-    (Link (Var "Top") (Link (Var "Odd") (Var "odd?"))).
-
-Definition test_num := succ_tm (three_tm).
-
-Compute get_wal (interp 10 (App test_even test_num)).
-Compute get_wal (interp 10 (App test_odd test_num)).
-Eval vm_compute in
-  let σ := interp 10 (Bind "n" test_num Mt) in
-  let w := interp 10 (App test_odd (Var "n")) in
-  get_wal (sem_link (link 10) σ w).
-End MutExample.
-
+(* Define : coinductive version of traces *)
+(* Define : strong bisimilarity between traces *)
+(* Define : depth-n approximation between traces *)
+(* Prove : strong bisimilarity ↔ equality of approximation for all n *)
+(* Conclusion : represent coinductive trace with a stream of "increasing" approximations *)
